src/Ex/Spec.v
@@ -1,15 +1,14 @@
 Require Import Bool Vector List String Peano_dec.
-Require Import Common FMap HVector ListSupport.
+Require Import Common FMap HVector IndexSupport.
 
 Set Implicit Arguments.
 
 (** Message Ids *)
 
-Definition getRq: IdxT := 0.
-Definition getRs: IdxT := 1.
-Definition setRq: IdxT := 2.
-Definition setRs: IdxT := 3.
-Definition evictRq: IdxT := 4.
-Definition evictRs: IdxT := 5.
-Definition specNumMsgIds := 6.
+Definition getRq: IdxT := 0~>0.
+Definition getRs: IdxT := 0~>1.
+Definition setRq: IdxT := 1~>0.
+Definition setRs: IdxT := 1~>1.
+Definition evictRq: IdxT := 2~>0.
+Definition evictRs: IdxT := 2~>1.
 
