src/Ex/SpecInds.v
@@ -1,0 +1,195 @@
+Require Import Bool Vector List String Peano_dec Omega.
+Require Import Common FMap HVector IndexSupport Syntax Semantics.
+Require Import Topology RqRsLang.
+
+Require Import Ex.Spec Ex.TopoTemplate.
+
+Set Implicit Arguments.
+
+Local Open Scope list.
+Local Open Scope hvec.
+Local Open Scope fmap.
+
+Lemma NoPrefix_NoDup:
+  forall inds, NoPrefix inds -> NoDup inds.
+Proof.
+  intros.
+  apply NoDup_nth_error; intros.
+  apply nth_error_Some in H0.
+  destruct (nth_error inds i) eqn:Hi; [clear H0|exfalso; auto].
+  apply eq_sym in H1.
+  destruct (eq_nat_dec i j); [assumption|exfalso].
+  specialize (H _ _ _ _ n Hi H1).
+  destruct H.
+  elim H.
+  apply IdxPrefix_refl.
+Qed.
+
+Lemma extendIdx_IdxDisj_congr:
+  forall bidx1 bidx2,
+    bidx1 ~*~ bidx2 ->
+    forall ext1 ext2,
+      bidx1~>ext1 ~*~ bidx2~>ext2.
+Proof.
+  unfold IdxDisj, extendIdx; intros; dest.
+  split.
+  - intro Hx; elim H.
+    red in Hx; dest.
+    destruct x; simpl in *.
+    + inv H1; apply IdxPrefix_refl.
+    + inv H1; exists (x ++ [ext1]); rewrite <-app_assoc; reflexivity.
+  - intro Hx; elim H0.
+    red in Hx; dest.
+    destruct x; simpl in *.
+    + inv H1; apply IdxPrefix_refl.
+    + inv H1; exists (x ++ [ext2]); rewrite <-app_assoc; reflexivity.
+Qed.
+
+Lemma NoPrefix_extendInds:
+  forall inds,
+    NoPrefix inds ->
+    forall e, NoPrefix (extendInds e inds).
+Proof.
+  unfold NoPrefix, extendInds; intros.
+  apply map_nth_error_inv in H1.
+  apply map_nth_error_inv in H2; dest; subst.
+  apply extendIdx_IdxDisj_congr.
+  eapply H; eauto.
+Qed.
+
+Section System.
+  Variable cinds: list IdxT.
+  Hypothesis (Hcinds: NoPrefix cinds).
+
+  Instance SpecOStateIfc: OStateIfc :=
+    {| ost_sz := 1;
+       ost_ty := [nat:Type]%vector |}.
+
+  Definition specIdx: IdxT := 0.
+  Definition specValueIdx: Fin.t 1 := Fin.F1.
+  Definition specOStatesInit: OStates :=
+    [specIdx <- hvcons 0 hvnil].
+  Definition specORqsInit: ORqs Msg :=
+    [specIdx <- []].
+
+  Section PerChn.
+    Variable eidx: IdxT.
+
+    Definition specGetRq: Rule :=
+      {| rule_idx := [0]~~eidx;
+         rule_precond :=
+           MsgsFrom [rqUpFrom eidx]
+           /\oprec MsgIdsFrom [getRq]
+           /\oprec RqAccepting;
+         rule_trs :=
+           fun ost orq mins =>
+             (ost, orq,
+              [(downTo eidx, {| msg_id := getRs;
+                                msg_type := MRs;
+                                msg_value := ost#[specValueIdx]
+                             |})])
+      |}.
+
+    Definition specSetRq: Rule :=
+      {| rule_idx := [1]~~eidx;
+         rule_precond :=
+           MsgsFrom [rqUpFrom eidx]
+           /\oprec MsgIdsFrom [setRq]
+           /\oprec RqAccepting;
+         rule_trs :=
+           fun (ost: OState) orq mins =>
+             ((hd_error mins)
+                >>=[ost] (fun idm =>
+                            ost+#[specValueIdx <- msg_value (valOf idm)]),
+              orq,
+              [(downTo eidx, {| msg_id := setRs;
+                                msg_type := MRs;
+                                msg_value := O |})])
+      |}.
+
+  End PerChn.
+
+  Definition specRulesI (eidx: IdxT): list Rule :=
+    [specGetRq eidx; specSetRq eidx].
+
+  Definition specRules (einds: list IdxT): list Rule :=
+    List.concat (map (fun eidx => specRulesI eidx) einds).
+
+  Hint Unfold specRulesI specRules: RuleConds.
+
+  Ltac disc_child_inds_NoPrefix :=
+    try match goal with
+        | [Hnp: NoPrefix ?inds, H0: ?n1 <> ?n2,
+           H1: nth_error ?inds ?n1 = Some _,
+           H2: nth_error ?inds ?n2 = Some _ |- _] =>
+          specialize (Hnp _ _ _ _ H0 H1 H2); destruct Hnp; auto
+        end.
+
+  Lemma specObj_rules_valid:
+    NoDup (map rule_idx (specRules (extendInds 0 cinds))).
+  Proof.
+    apply NoPrefix_extendInds with (e:= 0) in Hcinds.
+    solve_inds_NoDup disc_child_inds_NoPrefix.
+  Qed.
+
+  Definition specObj: Object :=
+    {| obj_idx := specIdx;
+       obj_rules := specRules (extendInds 0 cinds);
+       obj_rules_valid := specObj_rules_valid
+    |}.
+
+  Definition specMerqs: list IdxT :=
+    extendInds rqUpIdx (extendInds 0 cinds).
+
+  Definition specMerss: list IdxT :=
+    extendInds downIdx (extendInds 0 cinds).
+
+  Lemma spec_msg_inds_valid:
+    NoDup (specMerqs ++ specMerss).
+  Proof.
+    apply NoDup_DisjList.
+    - do 2 apply extendIdx_NoDup.
+      apply NoPrefix_NoDup; assumption.
+    - do 2 apply extendIdx_NoDup.
+      apply NoPrefix_NoDup; assumption.
+    - apply idx_DisjList_head.
+      eapply DisjList_SubList; [apply extendInds_idxHd_SubList|].
+      eapply DisjList_comm, DisjList_SubList; [apply extendInds_idxHd_SubList|].
+      solve_DisjList eq_nat_dec.
+  Qed.
+
+  Definition spec: System :=
+    {| sys_objs := [specObj];
+       sys_oinds_valid := ltac:(inds_valid_tac);
+       sys_minds := nil;
+       sys_merqs := specMerqs;
+       sys_merss := specMerss;
+       sys_msg_inds_valid := spec_msg_inds_valid;
+       sys_oss_inits := specOStatesInit;
+       sys_orqs_inits := specORqsInit
+    |}.
+
+End System.
+
+Section Facts.
+
+  Lemma specGetRq_in_specRules:
+    forall oidx einds,
+      In oidx einds ->
+      In (specGetRq oidx) (specRules einds).
+  Proof.
+    induction einds; simpl; intros; auto.
+    destruct H; subst; auto.
+  Qed.
+
+  Lemma specSetRq_in_specRules:
+    forall oidx einds,
+      In oidx einds ->
+      In (specSetRq oidx) (specRules einds).
+  Proof.
+    induction einds; simpl; intros; auto.
+    destruct H; subst; auto.
+  Qed.
+
+End Facts.
+
